Some refactoring.

Isabelle2/AbstractMultiPaxosR1.thy
@@ -5,8 +5,6 @@ begin
 text {*
 1) Acceptors vote for a suggestion, and leaders use the distributed implementation of the safe-at computation.
 2) Explicit 1b messages.
-3) Explicit learning.
-4) Catch-up.
 5) Localizing suggestions (the leader function).
 6) Explicit leadership acquisition.
 *}
@@ -17,13 +15,12 @@ record ('v,'a,'l) ampr1_state =
   vote :: "inst \<Rightarrow> 'a \<Rightarrow> bal \<rightharpoonup> 'v"
   suggestion :: "inst \<Rightarrow> bal \<rightharpoonup> 'v"
   onebs :: "'a \<Rightarrow> bal \<rightharpoonup> (inst \<rightharpoonup> ('v\<times>bal))"
-  learned :: "'l \<Rightarrow> inst \<rightharpoonup> 'v"
   leader :: "'a \<Rightarrow> bool"
 
 global_interpretation dsa:distributed_safe_at quorums ballot vote for quorums ballot vote 
   defines acc_max = dsa.acc_max and max_quorum_votes = dsa.max_quorum_votes .
 
-locale ampr1_ioa = IOA +
+locale ampr1_ioa =
   fixes quorums::"'a set set" and leader :: "bal \<Rightarrow> 'a"
   -- {* @{term leader} determines the leader of a ballot. *}
 begin
@@ -31,7 +28,7 @@ begin
 definition start where
   -- {* The initial state *}
   "start \<equiv> {\<lparr>propCmd = {}, ballot = (\<lambda> a . 0), vote = (\<lambda> i a . Map.empty), 
-    suggestion = \<lambda> i . Map.empty, onebs = \<lambda> a . Map.empty, learned = \<lambda> l . Map.empty,
+    suggestion = \<lambda> i . Map.empty, onebs = \<lambda> a . Map.empty,
     leader = \<lambda> a . leader 0 = a\<rparr>}"
 
 subsection {* The transitions *}
@@ -78,11 +75,7 @@ abbreviation chosen where
   "chosen s i v \<equiv> ballot_array.chosen quorums (vote s i) v"
 
 definition learn where
-  "learn l i v s s' \<equiv> chosen s i v \<and> s' = s\<lparr>learned := (learned s)(l := (learned s l)(i := Some v))\<rparr>"
-
-definition catch_up where
-  "catch_up l1 l2 i v s s' \<equiv> learned s l2 i = Some v
-    \<and> s' = s\<lparr>learned := (learned s)(l1 := (learned s l1)(i := Some v))\<rparr>"
+  "learn i v s s' \<equiv> chosen s i v \<and> s' = s"
 
 fun trans_rel where
   "trans_rel r (Propose c) r' = propose c r r'"
@@ -90,19 +83,17 @@ fun trans_rel where
     (\<exists> a b . join_ballot a b r r')
     \<or> (\<exists> a i v . do_vote a i v r r')
     \<or> (\<exists> a i b v . suggest a i b v r r')
-    \<or> (\<exists> l1 l2 i v . catch_up l1 l2 i v r r')
     \<or> (\<exists> a q . acquire_leadership a q r r'))"
-| "trans_rel r (Learn i v l) r' = learn l i v r r'"
+| "trans_rel r (Learn i v) r' = learn i v r r'"
 
 lemma trans_cases[consumes 1]:
   assumes "trans_rel r a r'"
   obtains 
   (propose) c where "propose c r r'"
-| (learn) l i v where "learn l i v r r'"
+| (learn) i v where "learn i v r r'"
 | (join_ballot) a b where "join_ballot a b r r'"
 | (do_vote) a i v where "do_vote a i v r r'"
 | (suggest) a i b v where "suggest a i b v r r'"
-| (catch_up) l1 l2 i v where "catch_up l1 l2 i v r r'"
 | (acquire) a q where "acquire_leadership a q r r'"
   using assms apply induct apply simp
   by (metis ampr1_ioa.trans_rel.simps(1) ampr1_ioa.trans_rel.simps(3) paxos_action.exhaust trans_rel.simps(2)) 
@@ -116,7 +107,7 @@ definition ioa where
   "ioa \<equiv> \<lparr>ioa.asig = paxos_asig, start = start, trans = trans\<rparr>"
 
 lemmas simps = ioa_def asig_def start_def trans_def propose_def join_ballot_def
-  do_vote_def learn_def suggest_def catch_up_def acquire_leadership_def
+  do_vote_def learn_def suggest_def acquire_leadership_def
 
 end
 
