Isabelle2/AbstractMultiPaxosR2Correctness.thy
@@ -2,22 +2,20 @@ theory AbstractMultiPaxosR2Correctness
 imports AbstractMultiPaxosR1 AbstractMultiPaxosR2 Simulations
 begin
 
-print_locale ampr2_ioa
-
-locale ampr2_proof = IOA + quorums quorums + ampr2_ioa quorums for
-     quorums :: "'a set set" +
-  fixes ampr2_ioa :: "(('v,'a,'l)ampr2_state, ('v,'a,'l)ampr1.action) ioa"
-  and ampr1_ioa :: "(('v,'a,'l)ampr1_state, ('v,'a,'l)ampr1.action) ioa"
-  defines "ampr2_ioa \<equiv> ioa" and "ampr1_ioa \<equiv> ampr1.ioa"
+locale ampr2_proof = IOA + quorums quorums + ampr2_ioa quorums leader 
+  + r1:ampr1_ioa quorums leader
+  for quorums :: "'a set set" and leader :: "bal \<Rightarrow> 'a" + 
+  fixes ampr2_ioa :: "(('v, 'a, 'l) ampr2_state, 'v paxos_action) ioa"
+    and ampr1_ioa :: "(('v, 'a, 'l) ampr1_state, 'v paxos_action) ioa"
+  defines "ampr2_ioa \<equiv> ioa" and "ampr1_ioa \<equiv> r1.ioa"
 begin
 
 definition ref_map where "ref_map s \<equiv> \<lparr>
   ampr1_state.propCmd = propCmd s,
   ampr1_state.ballot = ballot s,
-  ampr1_state.vote = (\<lambda> i a . vote s a i),
+  ampr1_state.vote = (\<lambda> i a . vote s $ a $ i),
   ampr1_state.suggestion = suggestion s,
   ampr1_state.onebs = onebs s,
-  ampr1_state.learned = learned s,
   ampr1_state.leader = ampr2_state.leader s\<rparr>"
 
 term "ampr1_ioa"
