Isabelle2/AbstractMultiPaxosR3_Code.thy
@@ -1,0 +1,38 @@
+theory AbstractMultiPaxosR3_Code
+imports AbstractMultiPaxosR3
+begin
+
+definition n :: nat where "n \<equiv> 3"
+  -- {* The number of processes *}
+
+definition accs where "accs \<equiv> {1..n}"
+  -- {* The set of acceptors *}
+
+definition leader where "leader (b::nat) \<equiv> (b mod n) + 1"
+  
+definition next_bal :: "nat \<Rightarrow> nat \<Rightarrow> nat" where "next_bal b a \<equiv> 
+  (b div n + 1) * n + a"
+  
+global_interpretation cq:card_quorums accs
+  defines qs = "cq.quorums" and nas = "cq.nas"
+  apply (unfold_locales)
+   apply (simp add: accs_def n_def)
+  apply (simp add: accs_def)
+  done
+
+global_interpretation my_amp_r3:amp_r3 leader next_bal accs qs 
+  defines start = my_amp_r3.global_start
+    and trans = my_amp_r3.trans_rel
+    and propose = my_amp_r3.propose
+    and try_acquire_leadership = my_amp_r3.try_acquire_leadership
+    and process_msg = my_amp_r3.process_msg
+    and local_start = my_amp_r3.local_start
+    and receive_fwd = my_amp_r3.receive_fwd
+    and receive_1a = my_amp_r3.receive_1a
+  .
+
+subsection {* Code generation *}
+
+export_code local_start propose try_acquire_leadership process_msg in Scala
+
+end
